Security.thy
@@ -5,7 +5,6 @@ begin
 locale security = rules 
 
 type_synonym ('a,'b) Trace = "('b \<times> 'b) set list" 
-type_synonym ('a,'b) LTrace = "('b set \<times> ('b \<times> 'b) set) list" 
 
 context security
 begin
@@ -27,26 +26,15 @@ definition ev :: "('a,'b) com \<Rightarrow> 'b \<Rightarrow> ('a,'b) Trace \<Rig
   ("\<langle>_,_\<rangle> \<rightarrow>\<^sup>*_ \<langle>_,_\<rangle>" [50,40,40] 70)
   where "\<langle>c,m\<rangle> \<rightarrow>\<^sup>*t \<langle>c',m'\<rangle> \<equiv> trace_mem m t m' \<and> c \<mapsto>\<^sup>*t c'"
 
-text \<open> trace as list of local steps in order to collect vc + beh \<close>
-
-inductive_set local_trace :: "(('a,'b) com \<times> ('a,'b) LTrace \<times> ('a,'b) com) set"
-  and local_trace_abv :: "('a,'b) com \<Rightarrow> ('a,'b) LTrace \<Rightarrow> ('a,'b) com \<Rightarrow> bool" 
-                                                                       ("_ \<mapsto>\<^sup>l\<^sup>*_ _" [50,40,40] 70)
-  where
-  "local_trace_abv P t P' \<equiv> (P, t, P') \<in> local_trace"
-  | none[intro]: "c \<mapsto>\<^sup>l\<^sup>*[] c" 
-  | sil[intro]: "c\<^sub>1 \<leadsto> c\<^sub>2 \<Longrightarrow> c\<^sub>2 \<mapsto>\<^sup>l\<^sup>*t c\<^sub>3 \<Longrightarrow> c\<^sub>1 \<mapsto>\<^sup>l\<^sup>*t c\<^sub>3"
-  | gex[intro]: "c\<^sub>1 \<mapsto>[\<alpha>',r,\<alpha>] c\<^sub>2 \<Longrightarrow> c\<^sub>2 \<mapsto>\<^sup>l\<^sup>*t c\<^sub>3 \<Longrightarrow> c\<^sub>1 \<mapsto>\<^sup>l\<^sup>*(strip_tag \<alpha>')#t c\<^sub>3"
-
-
 (*non-interference over all basic commands *)
 definition tag_basic
   where "tag_basic a \<alpha> \<equiv>  (tag a, \<alpha>)"
 
 definition sec_pres :: "('a,'b) com \<Rightarrow> 'b rel \<Rightarrow> bool"
-  where "sec_pres c S \<equiv> \<forall>\<alpha> r m\<^sub>1 m\<^sub>2 m\<^sub>1'. (strip_tag \<alpha>) \<in> obs_basics c \<longrightarrow> 
-                m\<^sub>1 \<in> (vc \<alpha>\<llangle>r\<rrangle>) \<longrightarrow> (m\<^sub>1,m\<^sub>2) \<in> S \<longrightarrow> (m\<^sub>1,m\<^sub>1') \<in> beh \<alpha>\<llangle>r\<rrangle> \<longrightarrow> 
-                               (\<exists>m\<^sub>2'. (m\<^sub>2,m\<^sub>2') \<in> beh \<alpha>\<llangle>r\<rrangle> \<and> (m\<^sub>1',m\<^sub>2') \<in> S)"
+  where 
+  "sec_pres c S \<equiv> \<forall>\<alpha> r m\<^sub>1 m\<^sub>2 m\<^sub>1'. 
+     ((beforeReord \<alpha> r) \<inter> (basics c) \<noteq> {}) \<longrightarrow> m\<^sub>1 \<in> vc \<alpha> \<longrightarrow> (m\<^sub>1,m\<^sub>2) \<in> S \<longrightarrow> 
+                             (m\<^sub>1,m\<^sub>1') \<in> beh \<alpha> \<longrightarrow> (\<exists>m\<^sub>2'. (m\<^sub>2,m\<^sub>2') \<in> beh \<alpha> \<and> (m\<^sub>1',m\<^sub>2') \<in> S)"
 
 (* non-interference over all traces *)
 
@@ -75,142 +63,47 @@ lemma trace_preE [elim]:
   obtains P\<^sub>2 where "P\<^sub>1 \<mapsto>\<^sup>*[x] P\<^sub>2" "P\<^sub>2 \<mapsto>\<^sup>*t P\<^sub>3"
   using assms by (metis append.simps(1) append.simps(2) trace_concatE)
 
-lemma basics_exec_step:
-  assumes "c \<mapsto>[\<alpha>'',r,\<alpha>] c'" 
-  shows "\<alpha> \<in> basics c"
-  using assms by induct auto
-
-(*
-lemma obs_basics_silent: 
-  assumes "P\<^sub>1 \<leadsto> P\<^sub>2"
-  shows "obs_basics P\<^sub>1 \<supseteq> obs_basics P\<^sub>2"
-  using assms basics_exec 
-proof (induct)
-  case (capS c c' k)
-  then show ?case
-    apply simp 
-    by blast
-next
-  case (capStep c \<alpha>' r \<alpha> c' s s')
-  have \<alpha>: "\<alpha>' = \<alpha>\<llangle>r\<rrangle>" using capStep lexecute_triple by auto
-  hence " basics c' \<subseteq>  basics c" using capStep by auto
-  hence " obs_basics c' \<subseteq>  obs_basics c" using capStep sledgehammer
-  hence "\<Union> (observable ` basics c') \<subseteq> \<Union> (observable ` basics c)" 
-  moreover have "\<exists>x\<in>basics c. popbasic' s s' \<alpha>' \<in> observable x"
-    unfolding overapprox_def 
-      
-      sorry
-  ultimately show ?case by simp
-qed auto
-*)
-
-
-(*
-
-lemma helpCap: 
-  assumes  "c \<mapsto>[\<alpha>',r,\<alpha>] c'" 
-  assumes  "c \<mapsto>[\<alpha>',r,\<alpha>] c' \<Longrightarrow> basics c' \<subseteq> basics c"
-  shows "obs_basics (Basic (popbasic' s s' \<alpha>') \<cdot> Capture s' c') \<subseteq> obs_basics (Capture s c)" 
-  using assms apply auto
-proof -
-  have a0:"\<exists>x\<in>obs_basics c. (poppred' s (vc \<alpha>'), poprel' s s' (beh \<alpha>')) \<in> observable x"
-  
-
-     sorry
-
-(*
-"\<exists>x\<in>obs_basics c. (poppred' s (vc \<alpha>'), poprel' s s' (beh \<alpha>')) \<in> observable x"
-"\<And>a b aa ba. (aa, ba) \<in> obs_basics c' \<Longrightarrow> (a, b) \<in> observable (aa, ba) \<Longrightarrow> 
-                                           \<exists>x\<in>obs_basics c. (a, b) \<in> observable x"
-*)
-
-
-lemma helpS: 
-  assumes "s \<in> S"
-  shows  "obs_basics (seq2com s) \<subseteq> (\<Union>s\<in>S. strip_tag_set (set s))"
-  sorry
-
-
-lemma basics_silent:
-  assumes "c \<leadsto> c'"
-  shows "obs_basics c \<supseteq> obs_basics c'"
-  using assms basics_exec 
-proof (induct)
-next 
-  case (bigc s S)
-  then show ?case by (simp add: helpS) 
-next
-  case (capS c c' k)
-  then show ?case apply simp by blast
-next
-  case (capStep c \<alpha>' r \<alpha> c' s s')
-  have a0: "\<alpha>' = \<alpha>\<llangle>r\<rrangle>" using capStep lexecute_triple by auto
-  hence a1: "basics c' \<subseteq>  basics c" using capStep by auto
-(*  have a2: "popbasic' s s' \<alpha>' \<in> popbasic ` basics c" sorry
-  have a3: "popbasic ` basics c' \<subseteq> popbasic ` basics c" sorry  *)
-  show ?case using helpCap using capStep.hyps using a1 by presburger
-qed auto
-*)
-
-text \<open>Identify all observable operations in a trace\<close>
-
-definition obs_atomics :: "('a,'b) com \<Rightarrow> ('b set \<times> 'b rel) set" 
-  where "obs_atomics c \<equiv> { \<alpha> | \<alpha> t c' . c \<mapsto>\<^sup>l\<^sup>*t c' \<and> \<alpha> \<in> set t }"
-
-
-definition obs_atomics' :: "('a,'b) com \<Rightarrow> ('b set \<times> 'b rel) set" 
-  where "obs_atomics c \<equiv> { \<alpha> | \<alpha> t c' . c \<mapsto>\<^sup>*t c' \<and> \<alpha> \<in> reorder_trace t c }"
-
-
-
-lemma basics_silent:
-  assumes "c \<leadsto> c'"
-  shows "obs_atomics c \<supseteq> obs_atomics c'"  sorry
-
-
-
-lemma obs_basics_lexec:
-  assumes "lexecute c \<alpha>' r \<alpha> c'" 
-  shows "obs_basics c \<supseteq> obs_basics c'"
-  using assms by (induct) auto
-
-lemma obs_basics_gex: 
-  assumes "gexecute c g c'" shows "obs_basics c \<supseteq> obs_basics c'"
-  using assms obs_basics_lexec by (induct) auto 
-
-
 lemma trace_basics: 
-  assumes "P\<^sub>1 \<mapsto>\<^sup>*t P\<^sub>2"
-  shows "obs_basics P\<^sub>1 \<supseteq> obs_basics P\<^sub>2"
-  using assms basics_silent obs_basics_gex by induct blast+
+  assumes "c \<mapsto>\<^sup>*t c'"
+  shows "basics c \<supseteq> basics c'"
+  using assms basics_silent
+proof (induct)
+  case (none c)
+  then show ?case by auto
+next
+  case (sil c\<^sub>1 c\<^sub>2 t c\<^sub>3)
+  then show ?case using basics_silent by blast
+next
+  case (gex c\<^sub>1 g c\<^sub>2 t c\<^sub>3)
+  then show ?case using basics_exec basics_simps(7,8) dual_order.trans basics_gexec by fast
+qed
 
-lemma basic_par_subset: (*Nick help with name please*)
-  assumes "gexecute c g c'" 
-  shows "basics c\<^sub>1 \<subseteq> basics (c\<^sub>1 || c\<^sub>2)" 
-        "basics c\<^sub>2 \<subseteq> basics (c\<^sub>1 || c\<^sub>2)" 
-  using assms by simp+
 
-(* ---not used:
 lemma something1: (*Nick help with name please*)
   assumes "gexecute c g c'" 
-  shows "\<exists>r \<alpha>. \<alpha> \<in> basics c \<and> g = beh \<alpha>\<llangle>r\<rrangle>"
-  using assms proof induct
-  case (thr c r \<alpha> c')
-  then show ?case using basics.simps(8) basics_lexec_prefix by blast
-qed auto
+  shows "\<exists>\<alpha> r. (beforeReord \<alpha> r) \<inter> (basics c) \<noteq> {} \<and> g = beh \<alpha>"
+  using assms proof induct  
+  case (thr c \<alpha>' r c')
+  then show ?case using basics_simps(8) basics_lexec by blast
+next
+  case (par1 c\<^sub>1 g c\<^sub>1' c\<^sub>2)
+  then show ?case using basics_simps(7) basics_lexec by blast
+next
+  case (par2 c\<^sub>2 g c\<^sub>2' c\<^sub>1)
+  then show ?case using basics_simps(7) basics_lexec by blast
+qed
 
 lemma something2: (*Nick help with name please*)
   assumes "c \<mapsto>\<^sup>*[g] c'"
-  shows "\<exists>r \<alpha>. \<alpha> \<in> basics c \<and> g = beh \<alpha>\<llangle>r\<rrangle>" 
+  shows "\<exists>r \<alpha>. (beforeReord \<alpha> r) \<inter> (basics c) \<noteq> {} \<and> g = beh \<alpha>" 
   using assms 
 proof (induct c "[g]" c')
   case (sil c\<^sub>1 c\<^sub>2 c\<^sub>3)
   then show ?case using basics_silent by blast
 next
   case (gex c\<^sub>1 c\<^sub>2 c\<^sub>3)
-  then show ?case using something1 by force
-qed
-*)
+  then show ?case using something1 by fast
+qed 
 
 
 lemma trace_rule_nil: 
@@ -222,16 +115,18 @@ lemma trace_rule_nil:
 lemma trace_rule: 
   assumes "c \<mapsto>\<^sup>*[g] c'"
   assumes "R,G \<turnstile> P {c} Q"
-  shows "\<exists>\<alpha> r M. (strip_tag \<alpha>) \<in> obs_basics c \<and> g = beh \<alpha>\<llangle>r\<rrangle> \<and> P \<subseteq> wp\<^sub>\<alpha> \<alpha>\<llangle>r\<rrangle> M \<and> guar\<^sub>\<alpha> \<alpha>\<llangle>r\<rrangle>  G \<and> R,G \<turnstile> M {c'} Q"
+  shows "\<exists>\<alpha> r M. (beforeReord \<alpha> r) \<inter> (basics c) \<noteq> {} \<and> 
+              g = beh \<alpha> \<and> P \<subseteq> wp\<^sub>\<alpha> \<alpha> M \<and> guar\<^sub>\<alpha> \<alpha>  G \<and> R,G \<turnstile> M {c'} Q"
   using assms 
 proof (induct c "[g]" c' arbitrary: P) 
   case (sil c\<^sub>1 c\<^sub>2 c\<^sub>3)
-  then show ?case using basics_silent rewrite_ruleI
-    by (metis (no_types, hide_lams) insert_subset subsetI subset_antisym)
+  then show ?case using basics_silent rewrite_ruleI 
+    by (smt (verit, ccfv_SIG) inf.absorb_iff1 inf_bot_right inf_left_commute)
 next
   case (gex c\<^sub>1 c\<^sub>2 c\<^sub>3)
-  then show ?case using trace_rule_nil gexecute_ruleI[OF gex(3,1)] sorry (*by fast *) 
+  then show ?case using basics_lexec trace_rule_nil gexecute_ruleI[OF gex(3,1)] sorry
 qed 
+
 
 lemma bisim_exists:
   assumes "sec_pres c S"
@@ -251,8 +146,8 @@ proof safe
   next
     case (2 m\<^sub>1 m\<^sub>1' g t m\<^sub>1'')
     then obtain c' where itm1: "c \<mapsto>\<^sup>*[g] c'" "c' \<mapsto>\<^sup>*t c\<^sub>1" by auto
-    then obtain P' r \<alpha> where itm2: "R,G \<turnstile> P' {c'} Q" "(strip_tag \<alpha>) \<in> obs_basics c" 
-      "g = beh \<alpha>\<llangle>r\<rrangle>" "P \<subseteq> wp\<^sub>\<alpha> \<alpha>\<llangle>r\<rrangle> P'"  using trace_rule[OF itm1(1) 2(5)] by blast
+    then obtain P' \<alpha> r where itm2: "R,G \<turnstile> P' {c'} Q" "(beforeReord \<alpha> r) \<inter> basics c \<noteq> {}" 
+      "g = beh \<alpha>" "P \<subseteq> wp\<^sub>\<alpha> \<alpha> P'"  using trace_rule[OF itm1(1) 2(5)] by blast
     hence itm6: "m\<^sub>1' \<in> P'" using 2(1,8) unfolding wp_def by blast                       
     then obtain m\<^sub>2' where itm3: "(m\<^sub>2,m\<^sub>2') \<in> g" "(m\<^sub>1',m\<^sub>2') \<in> S" using 2(1,4,6,8) itm2(2,3,4) 
       unfolding sec_pres_def wp_def by blast 
@@ -262,7 +157,7 @@ proof safe
       using 2(3)[OF itm4 itm2(1) itm3(2) itm1(2) itm6] by blast
     then show ?case using "2.prems"(4) itm3(1) by blast
    qed
-   thus ?thesis using that by (meson security.ev_def security_axioms) (*Could it be nicer?*)
+   thus ?thesis using that by (meson security.ev_def) (*Could it be nicer?*)
  qed
 
 theorem secure_bisim:
